Proof of correctness of the multisig contract

src/contracts_coq/multisig.v
@@ -3,6 +3,21 @@ Require Import macros.
 Import syntax.
 Import comparable.
 Require Import NArith.
+Require Import semantics.
+Import error.
+Require List.
+
+Print N.
+
+Section multisig.
+
+Context {get_contract_type : contract_constant -> error.M type} {nd : @node get_contract_type}.
+
+Definition instruction := @syntax.instruction get_contract_type.
+Definition data := @semantics.data get_contract_type.
+Definition stack := @semantics.stack get_contract_type.
+Definition eval {A B : stack_type} := @semantics.eval _ nd A B.
+Definition eval_precond := @semantics.eval_precond _ nd.
 
 Definition ADD_nat {S} : instruction (nat ::: nat ::: S) (nat ::: S) := ADD.
 
@@ -15,14 +30,16 @@ Definition parameter_ty := (pair
                 action_ty)
              (list_ (option_ signature))).
 
+Definition pack_ty := pair address (pair nat action_ty).
+
 
 Definition multisig : full_contract parameter_ty storage_ty :=
   (
-    UNPAIR ;; SWAP ;; DUP ;; DIP SWAP ;; (* ; < storage_ty ::: parameter_ty ::: storage_ty ::: nil > *)
+    UNPAIR ;; SWAP ;; DUP ;; DIP SWAP ;;
     DIP
       (
         UNPAIR ;;
-        DUP ;; @SELF parameter_ty _ ;; ADDRESS ;; PAIR ;;
+        DUP ;; @SELF _ parameter_ty _ ;; ADDRESS ;; PAIR ;;
         PACK ;;
         DIP ( UNPAIR ;; DIP SWAP ) ;; SWAP
       ) ;;
@@ -33,8 +50,8 @@ Definition multisig : full_contract parameter_ty storage_ty :=
     DIP SWAP ;; UNPAIR ;;
     DIP
       (
-        PUSH nat 0%N ;; SWAP ;;
-        ITER_list
+        PUSH nat (nat_constant 0%N) ;; SWAP ;;
+        ITER
           (
             DIP SWAP ;; SWAP ;;
             IF_CONS
@@ -45,7 +62,7 @@ Definition multisig : full_contract parameter_ty storage_ty :=
                       (
                         SWAP ;; DIIP ( DIP DUP ;; SWAP ) ;;
                         CHECK_SIGNATURE ;; ASSERT ;;
-                        PUSH nat 1%N ;; ADD_nat))
+                        PUSH nat (nat_constant 1%N) ;; ADD_nat))
                   ( SWAP ;; DROP )
               )
               (
@@ -57,7 +74,7 @@ Definition multisig : full_contract parameter_ty storage_ty :=
     ASSERT_CMPLE ;;
     DROP ;; DROP ;;
 
-    DIP ( UNPAIR ;; PUSH nat 1%N ;; ADD ;; PAIR ) ;;
+    DIP ( UNPAIR ;; PUSH nat (nat_constant 1%N) ;; ADD ;; PAIR ) ;;
 
     NIL operation ;; SWAP ;;
     IF_LEFT
@@ -65,3 +82,723 @@ Definition multisig : full_contract parameter_ty storage_ty :=
       ( IF_LEFT (SET_DELEGATE ;; CONS )
                 ( DIP ( SWAP ;; CAR ) ;; SWAP ;; PAIR ;; SWAP )) ;;
     PAIR ).
+
+Fixpoint check_all_signatures (sigs : list (option (data signature)))
+         (keys : list (data key))
+         (check_sig : data key -> data signature -> M Datatypes.bool) {struct keys} :=
+  match sigs, keys with
+  | nil, nil => true
+  | nil, cons _ _ => false
+  | cons _ _, nil => true
+  | cons (Some sig) sigs, cons k keys =>
+    match check_sig k sig with
+    | Failed _ _ => false
+    | Return _ b => andb b (check_all_signatures sigs keys check_sig)
+    end
+  | cons None sigs, cons _ keys =>
+    check_all_signatures sigs keys check_sig
+  end.
+
+Fixpoint count_signatures (sigs : list (option (data signature))) :=
+  match sigs with
+  | nil => 0%N
+  | cons None sigs => count_signatures sigs
+  | cons (Some _) sigs => (count_signatures sigs + 1)%N
+  end.
+
+
+Definition multisig_spec
+           (counter : N)
+           (action : data action_ty)
+           (sigs : list (option (data signature)))
+           (stored_counter : N)
+           (threshold : N)
+           (keys : list (data key))
+           (new_stored_counter : N)
+           (new_threshold : N)
+           (new_keys : list (data key))
+           (returned_operations : list (data operation)) :=
+  let params : data parameter_ty := ((counter, action), sigs) in
+  let storage : data storage_ty := (stored_counter, (threshold, keys)) in
+  exists self_contract self_address packed first_sigs remaining_sigs,
+    self nd parameter_ty = Return _ self_contract /\
+    address_ nd parameter_ty self_contract = Return _ self_address /\
+    pack nd pack_ty
+         (self_address, (counter, action)) = Return _ packed /\
+    counter = stored_counter /\
+    length first_sigs = length keys /\
+    sigs = (first_sigs ++ remaining_sigs)%list /\
+    check_all_signatures first_sigs keys
+                         (fun k sig => check_signature nd k sig packed) /\
+    (threshold <= count_signatures first_sigs)%N /\
+    match action with
+    | inl (amout, contr) =>
+      exists oper, transfer_tokens nd unit tt amout contr = Return _ oper /\
+                   new_stored_counter = (1 + stored_counter)%N /\
+                   new_threshold = threshold /\
+                   new_keys = keys /\
+                   returned_operations = (oper :: nil)%list
+    | inr (inl kh) => exists oper, set_delegate nd kh = Return _ oper /\
+                                   new_stored_counter = (1 + stored_counter)%N /\
+                                   new_threshold = threshold /\
+                                   new_keys = keys /\
+                                   returned_operations = (oper :: nil)%list
+    | inr (inr (nt, nks)) => new_stored_counter = (1 + stored_counter)%N /\
+                             new_threshold = nt /\
+                             new_keys = nks /\
+                             returned_operations = nil
+    end.
+
+
+Lemma forall_ex {A : Set} {phi psi : A -> Prop} :
+  (forall x, phi x <-> psi x) -> ((exists x, phi x) <-> (exists x, psi x)).
+Proof.
+  intro Hall.
+  split; intros (x, Hx); exists x; specialize (Hall x); intuition.
+Qed.
+
+Lemma ex_and_comm {A : Set} {P : Prop} {Q : A -> Prop} :
+  P /\ (exists x, Q x) <-> (exists x, P /\ Q x).
+Proof.
+  split.
+  - intros (p, (x, q)).
+    exists x.
+    auto.
+  - intros (x, (p, q)).
+    split.
+    + auto.
+    + exists x.
+      auto.
+Qed.
+
+Lemma ex_and_comm2 {A B : Set} {P : Prop} {Q : A -> B -> Prop} :
+  P /\ (exists x y, Q x y) <-> (exists x y, P /\ Q x y).
+Proof.
+  rewrite ex_and_comm.
+  apply forall_ex; intro x.
+  apply ex_and_comm.
+Qed.
+
+Lemma and_both {P Q R : Prop} : (Q <-> R) -> (P /\ Q <-> P /\ R).
+Proof.
+  intuition.
+Qed.
+
+Lemma ex_and_comm_both {A : Set} {P Q R}:
+  (Q <-> exists x : A, R x) ->
+  ((P /\ Q) <-> exists x : A, P /\ R x).
+Proof.
+  intro H.
+  transitivity (P /\ exists x, R x).
+  - apply and_both; assumption.
+  - apply ex_and_comm.
+Qed.
+
+Lemma ex_and_comm_both2 {A B : Set} {P Q R}:
+  (Q <-> exists (x : A) (y : B), R x y) ->
+  ((P /\ Q) <-> exists x y, P /\ R x y).
+Proof.
+  intro H.
+  transitivity (P /\ exists x y, R x y).
+  - apply and_both; assumption.
+  - apply ex_and_comm2.
+Qed.
+
+Lemma and_both_eq {X A B : Set} {P : Prop} {Q : X -> X -> Prop} {R : X -> X -> A -> B -> Prop} {x y : X}:
+  (Q x x <-> exists (a : A) (b : B), R x x a b) ->
+  ((x = y /\ Q x y) <-> (exists a b, x = y /\ R x y a b)).
+Proof.
+  intro H1.
+  split.
+  - intros (He, H2); subst x.
+    apply H1 in H2.
+    destruct H2 as (a, (b, H2)).
+    exists a; exists b.
+    split; [reflexivity|exact H2].
+  - intros (a, (b, (He, H2))).
+    subst x.
+    split; [reflexivity|].
+    apply H1.
+    exists a.
+    exists b.
+    exact H2.
+Qed.
+
+Lemma and_left {P Q R : Prop} : P -> (Q <-> R) -> ((P /\ Q) <-> R).
+Proof.
+  intuition.
+Qed.
+
+Lemma and_right {P Q R : Prop} : P -> (Q <-> R) -> (Q <-> (P /\ R)).
+Proof.
+  intuition.
+Qed.
+
+
+Lemma eqb_eq a c1 c2 :
+  BinInt.Z.eqb (comparison_to_int (compare a c1 c2)) Z0 = true <->
+  c1 = c2.
+Proof.
+  rewrite BinInt.Z.eqb_eq.
+  rewrite comparison_to_int_Eq.
+  apply comparable.compare_eq_iff.
+Qed.
+
+Lemma leb_le a c1 c2 :
+  BinInt.Z.leb (comparison_to_int (compare a c1 c2)) Z0 = true <->
+  (lt a c1 c2 \/ c1 = c2).
+Proof.
+  case_eq (compare a c1 c2); intro Hleb.
+  - rewrite compare_eq_iff in Hleb.
+    simpl.
+    generalize (BinInt.Z.leb_refl Z0).
+    intuition.
+  - simpl.
+    rewrite BinInt.Z.leb_le.
+    generalize (BinInt.Pos2Z.neg_is_nonpos 1).
+    unfold lt.
+    intuition.
+  - simpl.
+    rewrite Zbool.Zone_pos.
+    unfold lt.
+    split.
+    + discriminate.
+    + rewrite <- compare_eq_iff.
+      intros [|]; congruence.
+Qed.
+
+Lemma leb_gt a c1 c2 :
+  BinInt.Z.leb (comparison_to_int (compare a c1 c2)) Z0 = false <->
+  (gt a c1 c2).
+Proof.
+  unfold gt.
+  case_eq (compare a c1 c2); intro Hleb.
+  - simpl.
+    rewrite BinInt.Z.leb_refl.
+    split; discriminate.
+  - simpl.
+    assert (BinInt.Z.leb (Zneg 1) Z0 = true) as H.
+    + rewrite BinInt.Z.leb_le.
+      apply (BinInt.Pos2Z.neg_is_nonpos 1).
+    + rewrite H.
+      split; discriminate.
+  - simpl.
+    case_eq (BinInt.Z.leb (Zpos 1) Z0).
+    + intro H.
+      rewrite BinInt.Z.leb_le in H.
+      apply Zorder.Zle_not_lt in H.
+      destruct (H BinInt.Z.lt_0_1).
+    + intro; split; reflexivity.
+Qed.
+
+Definition multisig_head (then_ : instruction (nat ::: list_ key ::: list_ (option_ signature) ::: bytes ::: action_ty ::: storage_ty ::: nil) (pair (list_ operation) storage_ty ::: nil)) :
+  instruction (pair parameter_ty storage_ty ::: nil)
+              (pair (list_ operation) storage_ty ::: nil)
+:=
+    UNPAIR ;; SWAP ;; DUP ;; DIP SWAP ;;
+    DIP
+      (
+        UNPAIR ;;
+        DUP ;; @SELF _ parameter_ty _ ;; ADDRESS ;; PAIR ;;
+        PACK ;;
+        DIP ( UNPAIR ;; DIP SWAP ) ;; SWAP
+      ) ;;
+
+    UNPAIR ;; DIP SWAP ;;
+    ASSERT_CMPEQ ;;
+
+    DIP SWAP ;; UNPAIR ;; then_.
+
+Definition multisig_head_spec
+           (counter : N)
+           (action : data action_ty)
+           (sigs : list (option (data signature)))
+           (stored_counter : N)
+           (threshold : N)
+           (keys : list (data key))
+           (fuel : Datatypes.nat)
+           (then_ :
+              instruction
+                (nat ::: list_ key ::: list_ (option_ signature) ::: bytes :::
+                     action_ty ::: storage_ty ::: nil)
+                (pair (list_ operation) storage_ty ::: nil))
+           (psi : stack (pair (list_ operation) storage_ty ::: nil) -> Prop)
+  :=
+  let params : data parameter_ty := ((counter, action), sigs) in
+  let storage : data storage_ty := (stored_counter, (threshold, keys)) in
+  exists self_contract self_address packed,
+    self nd parameter_ty = Return _ self_contract /\
+    address_ nd parameter_ty self_contract = Return _ self_address /\
+    pack nd pack_ty
+         (self_address, (counter, action)) = Return _ packed /\
+    counter = stored_counter /\
+    precond (eval then_ fuel (threshold, (keys, (sigs, (packed, (action, (storage, tt))))))) psi.
+
+Ltac mysimpl :=
+  match goal with
+    |- ?g =>
+    match g with
+    | context c[semantics.eval_precond ?nd (S ?n) ?i ?psi] =>
+      is_var i ||
+             (let simplified := (eval simpl in (semantics.eval_precond nd (S n) i psi)) in
+              let full := context c[simplified] in
+              let final := eval cbv beta zeta iota in full in
+              change final)
+    end
+  end.
+
+Lemma fold_eval_precond fuel :
+  eval_precond_body nd (@semantics.eval_precond _ nd fuel) =
+  @semantics.eval_precond _ nd (S fuel).
+Proof.
+  reflexivity.
+Qed.
+
+Ltac more_fuel :=
+  match goal with
+    | Hfuel : (_ <= ?fuel) |- _ =>
+      destruct fuel as [|fuel];
+      [inversion Hfuel; fail
+      | apply le_S_n in Hfuel]
+  end.
+
+Lemma multisig_head_correct
+      (counter : N)
+      (action : data action_ty)
+      (sigs : list (option (data signature)))
+      (stored_counter : N)
+      (threshold : N)
+      (keys : list (data key))
+      (then_ :
+         instruction
+           (nat ::: list_ key ::: list_ (option_ signature) ::: bytes :::
+                action_ty ::: storage_ty ::: nil)
+           (pair (list_ operation) storage_ty ::: nil))
+      (psi : stack (pair (list_ operation) storage_ty ::: nil) -> Prop) :
+  let params : data parameter_ty := ((counter, action), sigs) in
+  let storage : data storage_ty := (stored_counter, (threshold, keys)) in
+  forall fuel, 9 <= fuel ->
+    (precond (eval (multisig_head then_) (10 + fuel) ((params, storage), tt)) psi)
+        <->
+    multisig_head_spec counter action sigs stored_counter threshold keys
+                       fuel then_ psi.
+Proof.
+  intros params storage fuel Hfuel.
+  unfold eval.
+  rewrite eval_precond_correct.
+  unfold multisig_head.
+  more_fuel.
+  unfold "+".
+  mysimpl.
+  apply forall_ex.
+  intro self; change (data (contract parameter_ty)) in self.
+  rewrite <- ex_and_comm2.
+  apply and_both.
+  apply forall_ex.
+  intro addr.
+  rewrite <- ex_and_comm.
+  apply and_both.
+  do 2 more_fuel; mysimpl.
+  apply forall_ex.
+  intro packed.
+  apply and_both.
+  do 6 more_fuel.
+  mysimpl.
+  case_eq (BinInt.Z.eqb (comparison_to_int (stored_counter ?= counter)%N) Z0).
+  - intro Heq.
+    apply (eqb_eq nat) in Heq.
+    symmetry in Heq.
+    apply (and_right Heq).
+    do 9 rewrite fold_eval_precond.
+    rewrite <- eval_precond_correct.
+    unfold eval.
+    reflexivity.
+  - intro Hneq.
+    split.
+    + intro H; inversion H.
+    + intros (Heq, _).
+      symmetry in Heq.
+      apply (eqb_eq nat) in Heq.
+      simpl in Heq.
+      exfalso.
+      congruence.
+Qed.
+
+Definition multisig_iter_body :
+  instruction
+    (key ::: nat ::: list_ (option_ signature) ::: bytes ::: action_ty :::
+         storage_ty ::: nil)
+    (nat ::: list_ (option_ signature) ::: bytes ::: action_ty :::
+         storage_ty ::: nil)
+  :=
+  (DIP SWAP ;; SWAP ;;
+       IF_CONS
+       (
+         IF_SOME
+           ( SWAP ;;
+                  DIP
+                  (
+                    SWAP ;; DIIP ( DIP DUP ;; SWAP ) ;;
+                         CHECK_SIGNATURE ;; ASSERT ;;
+                         PUSH nat (nat_constant 1%N) ;; ADD_nat))
+           ( SWAP ;; DROP )
+       )
+       (
+         FAIL
+       ) ;;
+       SWAP).
+
+Lemma multisig_iter_body_correct k n sigs packed
+      (st : stack (action_ty ::: storage_ty ::: nil)) fuel psi :
+    14 <= fuel ->
+    precond (eval multisig_iter_body fuel (k, (n, (sigs, (packed, st))))) psi
+    <->
+    match sigs with
+    | nil => false
+    | cons None sigs => psi (n, (sigs, (packed, st)))
+    | cons (Some sig) sigs =>
+      check_signature nd k sig packed = Return _ true /\
+      psi ((1 + n)%N, (sigs, (packed, st)))
+    end.
+Proof.
+  intro Hfuel.
+  unfold eval.
+  rewrite eval_precond_correct.
+  do 14 more_fuel.
+  mysimpl.
+  destruct sigs as [|[sig|] sigs].
+  - reflexivity.
+  - split.
+    + intros ([|], (Hckeck, H)).
+      * split; assumption.
+      * inversion H.
+    + intros (Hcheck, H).
+      exists true.
+      split; assumption.
+  - reflexivity.
+Qed.
+
+Definition multisig_iter :
+  instruction
+    (list_ key ::: nat ::: list_ (option_ signature) ::: bytes ::: action_ty :::
+         storage_ty ::: nil)
+    (nat ::: list_ (option_ signature) ::: bytes ::: action_ty :::
+         storage_ty ::: nil)
+  :=
+  ITER multisig_iter_body.
+
+(* Apres l'execution sur la pile (keys, n, sigs, packed, st), on renvoie (nb_de_signatures_valides + n, signatures exedentaires, packed, st) *)
+(* Invariant: all_keys = verified_keys @ remaining *)
+
+Lemma multisig_iter_correct keys n sigs packed
+      (st : stack (action_ty ::: storage_ty ::: nil)) fuel psi :
+    length keys * 14 + 1 <= fuel ->
+    precond (eval multisig_iter fuel (keys, (n, (sigs, (packed, st))))) psi <->
+    (exists first_sigs remaining_sigs,
+        length first_sigs = length keys /\
+        sigs = (first_sigs ++ remaining_sigs)%list /\
+        check_all_signatures
+          first_sigs keys (fun k sig => check_signature nd k sig packed) /\
+        psi ((count_signatures first_sigs + n)%N, (remaining_sigs, (packed, st)))).
+Proof.
+  unfold eval.
+  rewrite eval_precond_correct.
+  generalize n sigs packed fuel; clear n sigs packed fuel.
+  induction keys as [|key keys]; intros n sigs packed fuel Hfuel.
+  - simpl in Hfuel.
+    more_fuel.
+    mysimpl.
+    split.
+    + intro H.
+      exists nil.
+      exists sigs.
+      simpl.
+      intuition reflexivity.
+    + intros (first_sigs, (remaining_sigs, (Hlen, (Happ, (_, H))))).
+      simpl in Hlen.
+      apply List.length_zero_iff_nil in Hlen.
+      subst first_sigs.
+      simpl in Happ.
+      subst remaining_sigs.
+      exact H.
+  - simpl in Hfuel.
+    more_fuel.
+    change (13 + (length keys * 14 + 1) <= fuel) in Hfuel.
+    assert (length keys * 14 + 1 <= fuel) as Hfuel2 by (transitivity (13 + (length keys * 14 + 1)); [repeat constructor| apply Hfuel]).
+    mysimpl.
+    rewrite <- eval_precond_correct.
+    rewrite multisig_iter_body_correct.
+    + destruct sigs as [|[sig|] sigs].
+      * split; [intro H; inversion H|].
+        intros (first_sigs, (remaining_sigs, (Hlen, (Happ, _)))).
+        symmetry in Happ.
+        apply List.app_eq_nil in Happ.
+        destruct Happ as (Hfirst, _).
+        subst first_sigs.
+        simpl in Hlen.
+        discriminate.
+      * split.
+        -- intros (Hcheck, Hrec).
+           specialize (IHkeys (1 + n)%N sigs packed fuel Hfuel2).
+           rewrite IHkeys in Hrec.
+           destruct Hrec as (first_sigs, (remaining_sigs, (Hlen, (Happ, (Hchecks, H))))).
+           exists (Some sig :: first_sigs)%list.
+           exists remaining_sigs.
+           split ; [simpl; f_equal; assumption|].
+           subst sigs.
+           split ; [reflexivity|].
+           split.
+           ++ simpl.
+              rewrite Hcheck.
+              exact Hchecks.
+           ++ rewrite N.add_assoc in H.
+              exact H.
+        -- intros (first_sigs, (remaining_sigs, (Hlen, (Happ, (Hchecks, H))))).
+           destruct first_sigs as [|[first_sig|] first_sigs].
+           ++ simpl in Hlen.
+              discriminate.
+           ++ simpl in Happ.
+              injection Happ.
+              intro Hsigs; subst sigs.
+              intro Hsig; subst first_sig.
+              simpl in Hchecks.
+              destruct (check_signature nd key sig packed) as [|[|]].
+              ** inversion Hchecks.
+              ** simpl in Hchecks.
+                 split; [reflexivity|].
+                 apply (IHkeys _ _ _ _ Hfuel2).
+                 exists first_sigs; exists remaining_sigs.
+                 simpl in Hlen.
+                 apply NPeano.Nat.succ_inj in Hlen.
+                 split; [assumption|].
+                 split; [reflexivity|].
+                 split; [assumption|].
+                 simpl in H.
+                 rewrite N.add_assoc.
+                 exact H.
+              ** simpl in Hchecks.
+                 inversion Hchecks.
+           ++ simpl in Happ.
+              injection Happ.
+              discriminate.
+      * rewrite (IHkeys _ _ _ _ Hfuel2).
+        split;
+          intros (first_sigs, (remaining_sigs, (Hlen, (Happ, (Hchecks, H))))).
+        -- exists (None :: first_sigs)%list.
+           exists remaining_sigs.
+           split; [simpl; f_equal; exact Hlen|].
+           subst sigs.
+           split; [reflexivity|].
+           split; [exact Hchecks|].
+           exact H.
+        -- destruct first_sigs as [|[first_sig|] first_sigs].
+           ++ simpl in Hlen; discriminate.
+           ++ simpl in Happ; injection Happ; discriminate.
+           ++ exists first_sigs.
+              exists remaining_sigs.
+              simpl in Hlen.
+              apply NPeano.Nat.succ_inj in Hlen.
+              split; [assumption|].
+              simpl in Happ.
+              split; [injection Happ; auto|].
+              split; [exact Hchecks|].
+              exact H.
+    + transitivity (13 + (length keys * 14 + 1)).
+      * destruct (length keys).
+        -- simpl. constructor.
+        -- simpl. do 14 (apply Le.le_n_S).
+           apply le_0_n.
+      * assumption.
+Qed.
+
+Definition multisig_tail :
+  instruction
+    (nat ::: nat ::: list_ (option_ signature) ::: bytes ::: action_ty :::
+         storage_ty ::: nil)
+    (pair (list_ operation) storage_ty ::: nil) :=
+      ASSERT_CMPLE ;;
+    DROP ;; DROP ;;
+
+    DIP ( UNPAIR ;; PUSH nat (nat_constant 1%N) ;; ADD_nat ;; PAIR ) ;;
+
+    NIL operation ;; SWAP ;;
+    IF_LEFT
+      ( UNPAIR ;; UNIT ;; TRANSFER_TOKENS ;; CONS )
+      ( IF_LEFT (SET_DELEGATE ;; CONS )
+                ( DIP ( SWAP ;; CAR ) ;; SWAP ;; PAIR ;; SWAP )) ;;
+    PAIR.
+
+Lemma multisig_split : multisig = multisig_head (DIP (PUSH nat (nat_constant 0%N);; SWAP;; multisig_iter);; multisig_tail).
+Proof.
+  reflexivity.
+Qed.
+
+Lemma multisig_tail_correct
+      threshold n sigs packed action counter keys psi fuel :
+    13 <= fuel ->
+    precond (eval multisig_tail fuel (threshold, (n, (sigs, (packed, (action, ((counter, (threshold, keys)), tt))))))) psi <->
+    ((threshold <= n)%N /\
+     match action with
+    | inl (amout, contr) =>
+      exists oper, transfer_tokens nd unit tt amout contr = Return _ oper /\
+                   psi (((oper :: nil)%list, ((1 + counter)%N, (threshold, keys))), tt)
+    | inr (inl kh) =>
+      exists oper, set_delegate nd kh = Return _ oper /\
+                   psi (((oper :: nil)%list, ((1 + counter)%N, (threshold, keys))), tt)
+    | inr (inr (nt, nks)) =>
+      psi (nil, ((1 + counter)%N, (nt, nks)), tt)
+    end).
+Proof.
+  intro Hfuel.
+  change (data (list_ key)) in keys.
+  unfold eval.
+  rewrite eval_precond_correct.
+  unfold multisig_tail.
+  do 4 more_fuel.
+  mysimpl.
+  case_eq (BinInt.Z.leb (comparison_to_int (threshold ?= n)%N) Z0).
+  - intro Hle.
+    rewrite (leb_le nat) in Hle.
+    unfold lt, compare in Hle.
+    rewrite N.compare_lt_iff in Hle.
+    rewrite <- N.le_lteq in Hle.
+    apply (and_right Hle).
+    do 6 more_fuel.
+    mysimpl.
+    destruct action as [(amount, contract)|[delegate_key_hash|(new_threshold, new_keys)]].
+    + do 3 more_fuel.
+      reflexivity.
+    + more_fuel.
+      reflexivity.
+    + do 3 more_fuel.
+      reflexivity.
+  - do 3 more_fuel.
+    mysimpl.
+    intro Hle.
+    apply (leb_gt nat) in Hle.
+    rename Hle into Hgt.
+    unfold gt, compare in Hgt.
+    rewrite N.compare_gt_iff in Hgt.
+    split.
+    + intro H; inversion H.
+    + intros (Hle, _).
+      apply N.lt_nge in Hgt.
+      contradiction.
+Qed.
+
+Lemma multisig_correct
+      (counter : N)
+      (action : data action_ty)
+      (sigs : list (option (data signature)))
+      (stored_counter : N)
+      (threshold : N)
+      (keys : list (data key))
+      (new_stored_counter : N)
+      (new_threshold : N)
+      (new_keys : list (data key))
+      (returned_operations : list (data operation))
+      (fuel : Datatypes.nat) :
+  let params : data parameter_ty := ((counter, action), sigs) in
+  let storage : data storage_ty := (stored_counter, (threshold, keys)) in
+  let new_storage : data storage_ty := (new_stored_counter, (new_threshold, new_keys)) in
+  14 * length keys + 37 <= fuel ->
+  eval multisig fuel ((params, storage), tt) = Return _ ((returned_operations, new_storage), tt) <->
+  multisig_spec counter action sigs stored_counter threshold keys new_stored_counter new_threshold new_keys returned_operations.
+Proof.
+  intros params storage new_storage Hfuel.
+  rewrite return_precond.
+  rewrite multisig_split.
+  rewrite PeanoNat.Nat.add_comm in Hfuel.
+  do 10 more_fuel.
+  change (S (S (S (S (S (S (S (S (S (S fuel)))))))))) with (10 + fuel).
+  unfold params, storage.
+  rewrite multisig_head_correct.
+  - unfold multisig_head_spec, multisig_spec.
+    apply forall_ex; intro contract.
+    apply forall_ex; intro address.
+    apply forall_ex; intro packed.
+    apply ex_and_comm_both2.
+    apply ex_and_comm_both2.
+    apply ex_and_comm_both2.
+    apply ex_and_comm_both2.
+    clear params counter.
+    unfold eval.
+    rewrite eval_precond_correct.
+    more_fuel; mysimpl.
+    match goal with
+    | |- semantics.eval_precond nd fuel ?i ?t ?st <-> ?r =>
+      pose (t) as then_; change (semantics.eval_precond nd fuel i then_ st <-> r)
+    end.
+    more_fuel; mysimpl.
+    more_fuel; mysimpl.
+    more_fuel; mysimpl.
+    match goal with
+    | |- semantics.eval_precond nd fuel ?i ?t ?st <-> ?r =>
+      pose (t) as iter; change (semantics.eval_precond nd fuel i iter st <-> r)
+    end.
+    more_fuel; mysimpl.
+    subst iter.
+    rewrite <- eval_precond_correct.
+    rewrite multisig_iter_correct.
+    apply forall_ex; intro first_sigs.
+    apply forall_ex; intro remaining_sigs.
+    apply and_both.
+    apply and_both.
+    apply and_both.
+    unfold then_.
+    rewrite <- eval_precond_correct.
+    rewrite multisig_tail_correct.
+    rewrite N.add_0_r.
+    apply and_both.
+    destruct action as [(amount, contr)|[delegate_key_hash|(new_t, new_k)]].
+    + apply forall_ex; intro oper.
+      apply and_both.
+      split.
+      * intro H.
+        injection H.
+        intro; subst keys.
+        intro; subst threshold.
+        intro; subst new_stored_counter.
+        intro; subst returned_operations.
+        intuition reflexivity.
+      * intros (Hcounter, (Hthreshold, (Hkeys, Hoper))).
+        subst new_stored_counter; subst keys; subst threshold; subst returned_operations.
+        reflexivity.
+    + apply forall_ex; intro oper.
+      apply and_both.
+      split.
+      * intro H.
+        injection H.
+        intro; subst keys.
+        intro; subst threshold.
+        intro; subst new_stored_counter.
+        intro; subst returned_operations.
+        intuition reflexivity.
+      * intros (Hcounter, (Hthreshold, (Hkeys, Hoper))).
+        subst new_stored_counter; subst keys; subst threshold; subst returned_operations.
+        reflexivity.
+    + split.
+      * intro H.
+        injection H.
+        intro; subst new_keys.
+        intro; subst new_threshold.
+        intro; subst new_stored_counter.
+        intro; subst returned_operations.
+        intuition reflexivity.
+      * intros (Hcounter, (Hthreshold, (Hkeys, Hoper))).
+        subst new_stored_counter; subst new_keys; subst new_threshold; subst returned_operations.
+        reflexivity.
+    + do 4 apply Le.le_n_S.
+      refine (NPeano.Nat.le_trans _ _ _ _ Hfuel).
+      do 9 apply Le.le_n_S.
+      apply le_0_n.
+    + rewrite PeanoNat.Nat.add_comm.
+      apply Le.le_n_S.
+      refine (NPeano.Nat.le_trans _ _ _ _ Hfuel).
+      do 22 constructor.
+      rewrite PeanoNat.Nat.mul_comm.
+      constructor.
+  - refine (NPeano.Nat.le_trans _ _ _ _ Hfuel).
+    do 9 apply Le.le_n_S.
+    apply le_0_n.
+Qed.
